\documentclass[12pt]{article}
\usepackage{../../template}
\author{niceguy}
\title{Lecture 20}
\begin{document}
\maketitle

\section{Eigenvalues for second order ODEs}
We have
$$\vec{x}' = A\vec{x}, \vec{x} = \begin{bmatrix} y \\ y'\end{bmatrix}, A = \begin{bmatrix} 0 & 1 \\ -\frac{c}{a} & -\frac{b}{a}\end{bmatrix}$$
for
$$ay'' + by' + cy = 0$$
The characteristic equation is then
$$\lambda^2 + \frac{b}{a}\lambda + \frac{c}{a} = 0$$
The null space has a dimension of 1, as there is a nontrivial element, and $A \neq \vec{0}$. Considering the first row, we have the eigenvector
$$\vec{v} = \begin{bmatrix} 1 \\ \lambda\end{bmatrix}$$ 

\begin{ex}
	$$y'' + 5y' + 6y = 0$$
	The eigenvalues are -3, -2, with eigenvectors $\begin{bmatrix} 1 \\ -3\end{bmatrix}, \begin{bmatrix} 1 \\ -2\end{bmatrix}$.
	Then
	$$\vec{x}(t) = c_1e^{-3t}\begin{bmatrix} 1 \\ -3\end{bmatrix} + c_2e^{-2t} \begin{bmatrix} 1 \\ -2\end{bmatrix}$$
	So
	$$y(t) = c_1e^{-3t} + c_2e^{-2t}$$
\end{ex}

\begin{ex}
	$$y'' + y' + y = 0$$
	Then
	$$A = \begin{bmatrix} 0 & 1 \\ -1 & -1\end{bmatrix}$$
	The characteristic equation gives us
	$$\lambda^2 + \lambda + 1 = 0 \Rightarrow \lambda = \frac{-1\pm\sqrt{3}i}{2}$$
	And
	$$\vec{v} = \begin{bmatrix} 1 \\ \frac{-1+\sqrt{3}i}{2}\end{bmatrix}$$
	Giving us
	$$\vec{x}(t) = c_1e^{\mu t}[\cos(\nu t)\vec{a} - \sin(\nu t)\vec{b}] + c_2e^{\mu t}[\sin(\nu t)\vec{a} + \cos(\nu t)\vec{b}]$$
	Plugging in the values,
	$$y(t) = c_1e^{-0.5t}\cos\left(\frac{\sqrt{3}}{2}t\right) + c_2e^{-0.5t}\sin\left(\frac{\sqrt{3}}{2}t\right)$$
\end{ex}

From the above example, we know that the first component of the eigenvector never has an imaginary part, so in general,
$$y(t) = c_1e^{\mu t}\cos(\nu t) + c_2e^{\mu t}\sin(\nu t)$$
	
\begin{ex}
	$$y''-\frac{y'+1}{4}y = 0$$
	where
	$$A = \begin{bmatrix} 0 & 1 \\ -\frac{1}{4} & 1\end{bmatrix}$$
	Where we have $\lambda = \frac{1}{2}$ and $\vec{v} = \begin{bmatrix} 1 \\ \frac{1}{2}\end{bmatrix}$. Then generalised eigenvector is
	\begin{align*}
		(A-\lambda I)\vec{w} &= \vec{v} \\
		\begin{bmatrix} -\frac{1}{2} & 1 \\ -\frac{1}{4} & \frac{1}{2}\end{bmatrix}\vec{w} &= \begin{bmatrix} 1 \\ \frac{1}{2}\end{bmatrix} \\
		\vec{w} &= \begin{bmatrix} 0 \\1\end{bmatrix}
	\end{align*}
	Which gives us
	$$y(t) = c_1e^{0.5t} + c_2te^{0.5t}$$
\end{ex}

We know that in general,
\begin{align*}
	A - \lambda I &= \begin{bmatrix} 0 & 1 \\ -\frac{c}{a} & -\frac{b}{a}\end{bmatrix} + \begin{bmatrix} \frac{b}{2a} & 0 \\ 0 & \frac{b}{2a}\end{bmatrix} \\
		      &= \begin{bmatrix} \frac{b}{2a} & 1 \\ -\frac{c}{a} & -\frac{b}{2a}\end{bmatrix}
\end{align*}
So we know $\vec{w} = \begin{bmatrix} 0 \\ 1\end{bmatrix}$ by substitution (or, the second column is equal to $\begin{bmatrix} 1 \\ \lambda\end{bmatrix}$).
\end{document}
