\documentclass[12pt]{article}
\usepackage{../../template}
\author{niceguy}
\title{Lecture 22}
\begin{document}

\maketitle

\section{Reynolds Transport Theorem}

Derivation: Consider a one dimensional flow with one inlet and one outlet. \\
At time $t$,
$$B_\mathrm{sys}(t) = B_\mathrm{cv}(t)$$
As both the system and control volume are equivalent. \\
At time $t+\Delta t$,
$$B_\mathrm{sys}(t+\Delta t) = B_\mathrm{cv}(t+\Delta t) + \Delta B_\mathrm{out} - \Delta B_\mathrm{in}$$
As $B_\mathrm{sys}(t+\Delta t)$ contains some $B$ which has left the control volume, but it does not contain the new $B$ that has entered it. Then
\begin{align*}
	\frac{dB_\mathrm{sys}}{dt} &= \lim_{\Delta t \rightarrow 0} \frac{B_\mathrm{sys}(t+\Delta t) - B_\mathrm{sys}(t)}{\Delta t} \\
				   &= \lim_{\Delta t \rightarrow 0} \frac{B_\mathrm{cv}(t+\Delta t) + \Delta B_\mathrm{out} - \Delta B_\mathrm{in} - B_\mathrm{cv}(t)}{\Delta t} \\
				   &= \lim_{\Delta t \rightarrow 0} \frac{B_\mathrm{cv}(t+\Delta t)-B_\mathrm{cv}(t)}{\Delta t} + \dot{B}_\mathrm{out} - \dot{B}_\mathrm{in} \\
				   &= \frac{dB_\mathrm{cv}}{dt} + \dot{B}_\mathrm{out} - \dot{B}\mathrm{in}
\end{align*}

Derivation: General Case with multiple inlets and outlets, $\rho, V, b$ may not be unform across the inlet and outlet parts, and $\vec{v}$ may not be normal to the inlet and outlet cross-sections. \\
We define
$$d\vec{A} := dA\hat{n}$$
Then
$$dm = \rho\vec{v}\cdot d\vec{A}$$
so
$$\dot{B}_\mathrm{net} = \dot{B}_\mathrm{out} - \dot{B}_\mathrm{in} = \oiint_{cs} \rho b\vec{v}\cdot d\vec{A}$$
and finally
$$\frac{dB_\mathrm{sys}}{dt} = \frac{dB_\mathrm{cv}}{dt} + \oiint_{cs}\rho b\vec{v}\cdot d\vec{A}$$

\begin{ex}
	Derive the conservation of mass equation in Eulerian form using the RTT. \\
	In Lagrangian form: $\frac{dm_\mathrm{sys}}{dt} = 0$ \\
	In Eulerian form:
	$$\frac{dm_\mathrm{cs}}{dt} + \dot{m}_\mathrm{out}-\dot{m}_\mathrm{in} = 0$$
	Which can be rewritten as
	$$\frac{d}{dt} \iiint_{cv}\rho dV + \oiint_{cs}\rho\vec{v}\cdot d\vec{A} = 0$$
\end{ex}

\section{Momentum Equation}

Derivation: In Lagrangian form,
$$\sum \vec{F}_\mathrm{sys} = \frac{d}{dt}\vec{M} = \frac{d}{dt} \int_\mathrm{sys} \vec{v}\rho dV$$
Substituting RTT,
$$\sum \vec{F}_\mathrm{sys} = \frac{d}{dt}\vec{M}_\mathrm{cv} + \dot{\vec{M}}_\mathrm{net} = \frac{d}{dt} \iiint_\mathrm{cv} \vec{v}\rho dV + \oiint_\mathrm{cv} \vec{v}\left(\rho\vec{v}\cdot d\vec{A}\right)$$

\end{document}
